spec/design/ARM/ArchTypes_H.thy
@@ -19,72 +19,28 @@ imports
   State_H
   Hardware_H
   "../../../lib/Lib"
-  keywords "instantiation'" :: thy_decl
 begin
-
-ML
-  \<open>val _ =
-  Outer_Syntax.command @{command_keyword instantiation2'} "instantiate and prove type arity"
-   (Parse.opt_target -- Parse.multi_arity --| Parse.begin
-     >> (fn (opt_target, arities) => 
-          Toplevel.local_theory NONE opt_target (fn lthy =>
-            let
-              val thy = Proof_Context.theory_of lthy;
-              val lthy' = Class.instantiation_cmd arities thy;
-            in
-              lthy'
-            end)));
-\<close>
-
-ML \<open>
-val _ =
-  Outer_Syntax.command @{command_keyword instantiation'} "instantiate and prove type arity"
-   (Parse.opt_target -- Parse.multi_arity --| Parse.begin
-     >> (fn (opt_target, arities) => 
-            Toplevel.generic_theory (
-              (fn (Context.Theory thy) =>
-                    let
-                      val lthy = Class.instantiation_cmd arities thy;
-                      val gthy = Context.Proof lthy;
-                      val _ =
-                        (case Local_Theory.pretty lthy of
-                          [] => ()
-                        | prts => Output.state (Pretty.string_of (Pretty.chunks prts)));
-                    in gthy end
-              | (Context.Proof lthy) =>
-                     let
-                       val thy = Proof_Context.theory_of lthy;
-                       val lthy' = Class.instantiation_cmd arities thy;
-                       val gthy = Context.Proof lthy';
-                       val _ =
-                        (case Local_Theory.pretty lthy' of
-                          [] => ()
-                        | prts => Output.state (Pretty.string_of (Pretty.chunks prts)));
-                      in gthy end))));
-\<close>
-
-ML \<open>Local_Theory.init\<close>
 context ARM begin
-
-datatype apiobject_type = Foo
 
 (* apiobject_type instance proofs *)
 (*<*)
-instantiation' ARM.apiobject_type :: enum begin
-interpretation ARM .
-
+instantiation apiobject_type :: enum begin
 definition
   enum_apiobject_type: "enum_class.enum \<equiv> 
     [ 
-      Foo
+      Untyped,
+      TCBObject,
+      EndpointObject,
+      NotificationObject,
+      CapTableObject
     ]"
 
 
 definition
-  "enum_class.enum_all (P :: ARM.apiobject_type \<Rightarrow> bool) \<longleftrightarrow> Ball UNIV P"
+  "enum_class.enum_all (P :: apiobject_type \<Rightarrow> bool) \<longleftrightarrow> Ball UNIV P"
 
 definition
-  "enum_class.enum_ex (P :: ARM.apiobject_type \<Rightarrow> bool) \<longleftrightarrow> Bex UNIV P"
+  "enum_class.enum_ex (P :: apiobject_type \<Rightarrow> bool) \<longleftrightarrow> Bex UNIV P"
 
   instance
   apply intro_classes
